Changed the definitions in Reachability to have classtable as module parameter

Reachability.v
@@ -1,40 +1,37 @@
 From Celsius Require Export Trees.
 From Celsius Require Export Eval.
 From Celsius Require Export PartialMonotonicity.
-Require Import ssreflect ssrbool. (*
+Require Import ssreflect ssrbool. 
 
 Require Import List.
 Import ListNotations.
-Open Scope nat_scope. *)
+Open Scope nat_scope.
+Open Scope list_scope.
 
-(* Reserved Notation "σ ⊨ l1 ⇝ l2" (at level 80). *)
-Inductive reachability : ClassTable -> Store -> Loc -> Loc ->Prop :=
-|rch_heap  : forall ct l σ,  l < (dom σ) -> (reachability ct σ l l)
-|rch_trans : forall ct l0 l1 l2 C ω σ, (reachability ct σ l0 l1) -> (getObj σ l1 = Some (C, ω)) -> (exists f, (getVal ω f = Some l2)) -> (l2 < dom σ) -> (reachability ct σ l0 l2).
+Module Reachability.
+  Parameter ct: ClassTable.
 
-Search _ (_ (_,_)).
-Check fst.
-Notation "σct ⊨ l1 ⇝ l2" := (reachability (snd σct) (fst σct) l1 l2) (at level 80, l1 at level 99).
+  (* Reserved Notation "σ ⊨ l1 ⇝ l2" (at level 80). *)
+  Inductive reachability : Store -> Loc -> Loc ->Prop :=
+  |rch_heap  : forall l σ,  l < (dom σ) -> (reachability σ l l)
+  |rch_trans : forall l0 l1 l2 C ω σ, (reachability σ l0 l1) -> (getObj σ l1 = Some (C, ω)) -> (exists f, (getVal ω f = Some l2)) -> (l2 < dom σ) -> (reachability σ l0 l2).
 
-Check rch_heap.
-Check rch_trans.
+  Notation "σ ⊨ l1 ⇝ l2" := (reachability σ l1 l2) (at level 80, l1 at level 99).
+  Notation "σ ⊨ l : 'cold'" := (l < dom (σ: Store)) (at level 80, l at level 99).
+  Notation "σ ⊨ l : 'warm'" := (exists C ω args fields methods , (getObj σ l) = Some (C, ω) /\ ((ct C) = Some (class args fields methods)) /\ (length fields <= length ω)) (at level 80, l at level 99).
+  Notation "σ ⊨ l : 'hot'"  := (forall (l': Loc), σ ⊨ l ⇝ l' -> (σ ⊨ l' : cold)) (at level 80, l at level 99).
 
-Lemma reachability_trans: (forall ct σ l1 l2 l3, ((σ, ct) ⊨ l1 ⇝ l2) -> ((σ, ct) ⊨ l2 ⇝ l3) -> ((σ, ct) ⊨ l1 ⇝ l3)).
-Proof.
-  intros ct σ l1 l2 l3 H1 H2.
-  induction H2 => //. 
-  apply (rch_trans ct0 l1 l2 l3 C ω σ0 (IHreachability H1) H H0 H3). 
-Qed.
-
-Notation "σct ⊨ l : 'cold'" := (l < dom (fst σct)) (at level 80, l at level 99).
-Notation "σct ⊨ l : 'warm'" := (exists C ω args fields methods , (getObj (fst σct) l) = Some (C, ω) /\ (((snd σct) C) = Some (class args fields methods)) /\ (length fields <= length ω)) (at level 80, l at level 99).
-Notation "σct ⊨ l : 'hot'"  := (forall l', (σct ⊨ l ⇝ l') -> (σct ⊨ l' : warm)) (at level 80, l at level 99).
-
-
-Lemma reachability_hot: forall (ct: ClassTable) (σ: Store) (l l': Loc), (σ, ct) ⊨ l: hot -> (σ, ct) ⊨ l ⇝ l' -> (σ, ct) ⊨ l': hot.
-Proof.
-  intros ct σ l l' H1 H2 l'' H3.
-  apply (H1 l'' ((reachability_trans _ _ _ _ _) H2 H3)).
-Qed. 
-                                             
-              
+  
+  Lemma reachability_trans: (forall σ l1 l2 l3, (σ ⊨ l1 ⇝ l2) -> (σ ⊨ l2 ⇝ l3) -> (σ ⊨ l1 ⇝ l3)).
+  Proof.
+    intros σ l1 l2 l3 H1 H2.
+    induction H2 => //. 
+    apply (rch_trans l1 l2 l3 C ω σ (IHreachability H1) H H0 H3). 
+  Qed.
+  Lemma reachability_hot: forall (σ: Store) (l l': Loc), σ ⊨ l: hot -> σ ⊨ l ⇝ l' -> σ ⊨ l': hot.
+  Proof.
+    intros σ l l' H1 H2 l'' H3.
+    apply (H1 l'' ((reachability_trans _ _ _ _) H2 H3)).
+  Qed. 
+  
+End Reachability.              
